Split off lemmas about [InlineConst]

src/Reflection/InlineWf.v
@@ -1,8 +1,8 @@
-(** * Linearize: Place all and only operations in let binders *)
+(** * Inline: Remove some [Let] expressions *)
 Require Import Crypto.Reflection.Syntax.
 Require Import Crypto.Reflection.WfProofs.
-Require Import Crypto.Reflection.Linearize.
-Require Import Crypto.Util.Tactics Crypto.Util.Sigma.
+Require Import Crypto.Reflection.Inline.
+Require Import Crypto.Util.Tactics Crypto.Util.Sigma Crypto.Util.Prod.
 
 Local Open Scope ctype_scope.
 Section language.
@@ -47,22 +47,13 @@ Section language.
       end.
     Local Ltac t_fin tac := repeat t_fin_step tac.
 
-    Lemma wff_let_bind_const G {t} v {tC} eC1 eC2
-      : (forall (x1 : interp_flat_type_gen var1 t) (x2 : interp_flat_type_gen var2 t),
-            wff (flatten_binding_list base_type_code x1 x2 ++ G) (eC1 x1) (eC2 x2))
-        -> @wff var1 var2 G tC (let_bind_const v eC1) (let_bind_const v eC2).
-    Proof.
-      revert G tC eC1 eC2; induction t; t_fin idtac.
-    Qed.
-
-    Local Hint Resolve wff_let_bind_const.
     Local Hint Constructors Syntax.wff.
     Local Hint Resolve List.in_app_or List.in_or_app.
 
     Local Ltac small_inversion_helper wf G0 e2 :=
       let t0 := match type of wf with wff (t:=?t0) _ _ _ => t0 end in
       let e1 := match goal with
-                | |- context[wff G0 (under_letsf ?e1 _) (under_letsf e2 _)] => e1
+                | |- context[wff _ (inline_constf ?e1) (inline_constf e2)] => e1
                 end in
       pattern G0, t0, e1, e2;
       lazymatch goal with
@@ -108,79 +99,68 @@ Section language.
                           | _ => fun _ p => p
                           end) ]
       end.
-    Fixpoint wff_under_letsf G {t} e1 e2 {tC} eC1 eC2
-             (wf : @wff var1 var2 G t e1 e2)
-             (H : forall (x1 : interp_flat_type_gen var1 t) (x2 : interp_flat_type_gen var2 t),
-                 wff (flatten_binding_list base_type_code x1 x2 ++ G) (eC1 x1) (eC2 x2))
-             {struct e1}
-      : @wff var1 var2 G tC (under_letsf e1 eC1) (under_letsf e2 eC2).
-    Proof.
-      revert H.
-      set (e1v := e1) in *.
-      destruct e1 as [ | | ? ? ? args | tx ex tC0 eC0 | ? ex ? ey ];
-        [ clear wff_under_letsf
-        | clear wff_under_letsf
-        | clear wff_under_letsf
-        | generalize (fun G => match e1v return match e1v with Let _ _ _ _ => _ | _ => _ end with
-                            | Let _ ex _ eC => wff_under_letsf G _ ex
-                            | _ => I
-                            end);
-          generalize (fun G => match e1v return match e1v with
-                                                | Let tx0 _ tC1 e0 => (* 8.4's type inferencer is broken, so we copy/paste the term from 8.5.  This entire clause could just be [_], if Coq 8.4 worked *)
-                                                  forall (x : @interp_flat_type_gen base_type_code var1 tx0) (e3 : exprf tC1)
-                                                         (tC2 : flat_type) (eC3 : @interp_flat_type_gen base_type_code var1 tC1 -> exprf tC2)
-                                                         (eC4 : @interp_flat_type_gen base_type_code var2 tC1 -> exprf tC2),
-                                                    wff G (e0 x) e3 ->
-                                                    (forall (x1 : @interp_flat_type_gen base_type_code var1 tC1)
-                                                            (x2 : @interp_flat_type_gen base_type_code var2 tC1),
-                                                        wff (@flatten_binding_list base_type_code var1 var2 tC1 x1 x2 ++ G) (eC3 x1) (eC4 x2)) ->
-                                                    wff G (@under_letsf base_type_code interp_base_type op var1 tC1 (e0 x) tC2 eC3)
-                                                        (@under_letsf base_type_code interp_base_type op var2 tC1 e3 tC2 eC4)
-                                                | _ => _ end with
-                               | Let _ ex tC' eC => fun x => wff_under_letsf G tC' (eC x)
-                               | _ => I
-                               end);
-          clear wff_under_letsf
-        | generalize (fun G => match e1v return match e1v with Pair _ _ _ _ => _ | _ => _ end with
-                            | Pair _ ex _ ey => wff_under_letsf G _ ex
-                            | _ => I
-                            end);
-          generalize (fun G => match e1v return match e1v with Pair _ _ _ _ => _ | _ => _ end with
-                            | Pair _ ex _ ey => wff_under_letsf G _ ey
-                            | _ => I
-                            end);
-          clear wff_under_letsf ];
-        revert eC1 eC2;
-        (* alas, Coq's refiner isn't smart enough to figure out these small inversions for us *)
-        small_inversion_helper wf G e2;
-        t_fin idtac.
-    Qed.
 
-    Local Hint Resolve wff_under_letsf.
     Local Hint Constructors or.
     Local Hint Extern 1 => progress unfold List.In in *.
     Local Hint Resolve wff_in_impl_Proper.
     Local Hint Resolve wff_SmartVar.
+    Local Hint Resolve wff_SmartConst.
 
-    Lemma wff_linearizef G {t} e1 e2
-      : @wff var1 var2 G t e1 e2
-        -> @wff var1 var2 G t (linearizef e1) (linearizef e2).
+    Fixpoint wff_inline_constf {t} e1 e2 G G'
+             (H : forall t x x', List.In (existT (fun t : base_type_code => (exprf t * exprf t)%type) t (x, x')) G'
+                            -> wff G x x')
+             (wf : wff G' e1 e2)
+             {struct e1}
+      : @wff var1 var2 G t (inline_constf e1) (inline_constf e2).
     Proof.
-      induction 1; t_fin ltac:(apply wff_under_letsf).
-    Qed.
-
-    Local Hint Resolve wff_linearizef.
-
-    Lemma wf_linearize G {t} e1 e2
-      : @wf var1 var2 G t e1 e2
-        -> @wf var1 var2 G t (linearize e1) (linearize e2).
-    Proof.
-      induction 1; t_fin idtac.
-    Qed.
+      (*revert H.
+      set (e1v := e1) in *.
+      destruct e1 as [ | | ? ? ? args | tx ex tC0 eC0 | ? ex ? ey ];
+        [ clear wff_inline_constf
+        | clear wff_inline_constf
+        | generalize (match e1v return match e1v with Let _ _ _ _ => _ | _ => _ end with
+                      | Op _ _ _ args => wff_inline_constf _ args
+                      | _ => I
+                      end);
+          clear wff_inline_constf
+        | generalize (match e1v return match e1v with Let _ _ _ _ => _ | _ => _ end with
+                      | Let _ ex _ eC => wff_inline_constf _ ex
+                      | _ => I
+                      end);
+          generalize (match e1v return match e1v with Let _ _ _ _ => _ | _ => _ end with
+                      | Let _ ex _ eC => fun x => wff_inline_constf _ (eC x)
+                      | _ => I
+                      end);
+          clear wff_inline_constf
+        | generalize (match e1v return match e1v with Let _ _ _ _ => _ | _ => _ end with
+                      | Pair _ ex _ ey => wff_inline_constf _ ex
+                      | _ => I
+                      end);
+          generalize (match e1v return match e1v with Let _ _ _ _ => _ | _ => _ end with
+                      | Pair _ ex _ ey => wff_inline_constf _ ey
+                      | _ => I
+                      end);
+          clear wff_inline_constf ];
+        revert G;
+        (* alas, Coq's refiner isn't smart enough to figure out these small inversions for us *)
+        small_inversion_helper wf G' e2;
+        t_fin idtac;
+        repeat match goal with
+               | [ H : context[(_ -> wff _ (inline_constf ?e) (inline_constf _))%type], e2 : exprf _ |- _ ]
+                 => is_var e; not constr_eq e e2; specialize (H e2)
+               | [ H : context[wff _ (@inline_constf ?A ?B ?C ?D ?E ?e) _] |- context[match @inline_constf ?A ?B ?C ?D ?E ?e with _ => _ end] ]
+                 => destruct (@inline_constf A B C D E e)
+               | [ H : context[wff _ _ (@inline_constf ?A ?B ?C ?D ?E ?e)] |- context[match @inline_constf ?A ?B ?C ?D ?E ?e with _ => _ end] ]
+                 => destruct (@inline_constf A B C D E e)
+               | [ IHwf : forall x y : list _, _, H1 : forall z : _, _, H2 : wff _ _ _ |- _ ]
+                 => solve [ specialize (IHwf _ _ H1 H2); inversion IHwf ]
+               | [ |- wff _ _ _ ] => constructor
+               end.
+      3:t_fin idtac.
+      4:t_fin idtac.
+      { match goal with
+        | [ H : _ |- _ ] => eapply H; [ | solve [ eauto ] ]; t_fin idtac
+        end. }*)
+    Abort.
   End with_var.
-
-  Lemma Wf_Linearize {t} (e : Expr t) : Wf e -> Wf (Linearize e).
-  Proof.
-    intros wf var1 var2; apply wf_linearize, wf.
-  Qed.
 End language.
