src/Reflection/Inline.v
@@ -1,0 +1,50 @@
+(** * Inline: Remove some [Let] expressions *)
+Require Import Crypto.Reflection.Syntax.
+Require Import Crypto.Util.Tactics.
+
+Local Open Scope ctype_scope.
+Section language.
+  Context (base_type_code : Type).
+  Context (interp_base_type : base_type_code -> Type).
+  Context (op : flat_type base_type_code -> flat_type base_type_code -> Type).
+
+  Local Notation flat_type := (flat_type base_type_code).
+  Local Notation type := (type base_type_code).
+  Let Tbase := @Tbase base_type_code.
+  Local Coercion Tbase : base_type_code >-> Syntax.flat_type.
+  Let interp_type := interp_type interp_base_type.
+  Let interp_flat_type := interp_flat_type_gen interp_base_type.
+  Local Notation Expr := (@Expr base_type_code interp_base_type op).
+
+  Section with_var.
+    Context {var : base_type_code -> Type}.
+    Local Notation exprf := (@exprf base_type_code interp_base_type op).
+    Local Notation expr := (@expr base_type_code interp_base_type op).
+
+    Fixpoint inline_constf {t} (e : @exprf (@exprf var) t) : @exprf var t
+      := match e in Syntax.exprf _ _ _ t return @exprf var t with
+         | Let _ ex tC eC
+           => match @inline_constf _ ex in Syntax.exprf _ _ _ t' return (interp_flat_type_gen _ t' -> @exprf var tC) -> @exprf var tC with
+              | Const _ x => fun eC => eC (SmartConst (op:=op) (var:=var) x)
+              | ex => fun eC => Let ex (fun x => eC (SmartVarVar x))
+              end (fun x => @inline_constf _ (eC x))
+         | Var _ x => x
+         | Const _ x => Const x
+         | Pair _ ex _ ey => Pair (@inline_constf _ ex) (@inline_constf _ ey)
+         | Op _ _ op args => Op op (@inline_constf _ args)
+         end.
+
+    Fixpoint inline_const {t} (e : @expr (@exprf var) t) : @expr var t
+      := match e in Syntax.expr _ _ _ t return @expr var t with
+         | Return _ x => Return (inline_constf x)
+         | Abs _ _ f => Abs (fun x => @inline_const _ (f (Var x)))
+         end.
+  End with_var.
+
+  Definition InlineConst {t} (e : Expr t) : Expr t
+    := fun var => inline_const (e _).
+End language.
+
+Global Arguments inline_constf {_ _ _ _ _} _.
+Global Arguments inline_const {_ _ _ _ _} _.
+Global Arguments InlineConst {_ _ _ _} _ var.
