src/Reflection/WfProofs.v
@@ -1,5 +1,5 @@
 Require Import Crypto.Reflection.Syntax.
-Require Import Crypto.Util.Tactics.
+Require Import Crypto.Util.Tactics Crypto.Util.Sigma Crypto.Util.Prod.
 
 Local Open Scope ctype_scope.
 Section language.
@@ -36,5 +36,54 @@ Section language.
                | _ => solve [ intuition eauto ]
                end.
     Qed.
+
+    Local Hint Resolve List.in_app_or List.in_or_app.
+    Local Hint Extern 1 => progress unfold List.In in *.
+    Local Hint Resolve wff_in_impl_Proper.
+
+    Lemma wff_SmartVar {t} x1 x2
+      : @wff var1 var2 (flatten_binding_list base_type_code x1 x2) t (SmartVar x1) (SmartVar x2).
+    Proof.
+      unfold SmartVar.
+      induction t; simpl; constructor; eauto.
+    Qed.
+
+    Local Hint Resolve wff_SmartVar.
+
+    Lemma wff_Const_eta G {A B} v1 v2
+      : @wff var1 var2 G (Prod A B) (Const v1) (Const v2)
+        -> (@wff var1 var2 G A (Const (fst v1)) (Const (fst v2))
+           /\ @wff var1 var2 G B (Const (snd v1)) (Const (snd v2))).
+    Proof.
+      intro wf.
+      assert (H : Some v1 = Some v2).
+      { refine match wf in @Syntax.wff _ _ _ _ _ G t e1 e2 return invert_Const e1 = invert_Const e2 with
+               | WfConst _ _ _ => eq_refl
+               | _ => eq_refl
+               end. }
+      inversion H; subst; repeat constructor.
+    Qed.
+
+    Definition wff_Const_eta_fst G {A B} v1 v2 H
+      := proj1 (@wff_Const_eta G A B v1 v2 H).
+    Definition wff_Const_eta_snd G {A B} v1 v2 H
+      := proj2 (@wff_Const_eta G A B v1 v2 H).
+
+    Local Hint Resolve wff_Const_eta_fst wff_Const_eta_snd.
+
+    Lemma wff_SmartConst G {t t'} v1 v2 x1 x2
+          (Hin : List.In (existT (fun t : base_type_code => (@exprf var1 t * @exprf var2 t)%type) t (x1, x2))
+                         (flatten_binding_list base_type_code (SmartConst v1) (SmartConst v2)))
+          (Hwf : @wff var1 var2 G t' (Const v1) (Const v2))
+      : @wff var1 var2 G t x1 x2.
+    Proof.
+      induction t'. simpl in *.
+      { intuition (inversion_sigma; inversion_prod; subst; eauto). }
+      { unfold SmartConst in *; simpl in *.
+        apply List.in_app_iff in Hin.
+        intuition (inversion_sigma; inversion_prod; subst; eauto). }
+    Qed.
+
+    Local Hint Resolve wff_SmartConst.
   End with_var.
 End language.
